examples/CCS/ObsCongrLawsScript.sml
@@ -5,10 +5,8 @@
 
 open HolKernel Parse boolLib bossLib;
 
-open CCSLib CCSTheory;
-open StrongEQTheory StrongEQLib StrongLawsTheory;
-open WeakEQTheory WeakEQLib WeakLawsTheory;
-open ObsCongrTheory ObsCongrLib;
+open CCSLib CCSTheory StrongEQTheory StrongEQLib StrongLawsTheory
+     WeakEQTheory WeakEQLib WeakLawsTheory ObsCongrTheory ObsCongrLib;
 
 val _ = new_theory "ObsCongrLaws";
 
@@ -121,7 +119,7 @@ val OBS_PAR_TAU_TAU = save_thm (
  *)
 val OBS_PAR_PREF_NO_SYNCR = save_thm (
    "OBS_PAR_PREF_NO_SYNCR",
-    STRIP_FORALL_RULE ((DISCH ``~((l :'b Label) = COMPL l')``) o
+    STRIP_FORALL_RULE ((DISCH ``~((l :'a Label) = COMPL l')``) o
                        (STRIP_FORALL_RULE (MATCH_MP STRONG_IMP_OBS_CONGR)) o
                        UNDISCH)
                       STRONG_PAR_PREF_NO_SYNCR);
@@ -138,7 +136,7 @@ val OBS_PAR_PREF_NO_SYNCR = save_thm (
  *)
 val OBS_PAR_PREF_SYNCR = save_thm (
    "OBS_PAR_PREF_SYNCR",
-    STRIP_FORALL_RULE ((DISCH ``((l :'b Label) = COMPL l')``) o
+    STRIP_FORALL_RULE ((DISCH ``((l :'a Label) = COMPL l')``) o
                        (STRIP_FORALL_RULE (MATCH_MP STRONG_IMP_OBS_CONGR)) o
                        UNDISCH)
                       STRONG_PAR_PREF_SYNCR);
@@ -194,15 +192,15 @@ val OBS_RESTR_PREFIX_TAU = save_thm (
 val OBS_RESTR_PR_LAB_NIL = save_thm (
    "OBS_RESTR_PR_LAB_NIL",
    ((Q.GENL [`l`, `L`]) o
-    (DISCH ``(l :'b Label) IN L \/ (COMPL l) IN L``) o
+    (DISCH ``(l :'a Label) IN L \/ (COMPL l) IN L``) o
     (Q.GEN `E`) o
     UNDISCH)
        (IMP_TRANS
-           (DISCH ``(l :'b Label) IN L \/ (COMPL l) IN L``
+           (DISCH ``(l :'a Label) IN L \/ (COMPL l) IN L``
             (Q.SPEC `E`
              (UNDISCH
               (Q.SPECL [`l`, `L`] STRONG_RESTR_PR_LAB_NIL))))
-           (SPECL [``restr (L :'b Label set) (prefix (label l) E)``, ``nil``]
+           (SPECL [``restr (L :'a Label set) (prefix (label l) E)``, ``nil``]
                   STRONG_IMP_OBS_CONGR)));
 
 (* Prove OBS_RESTR_PREFIX_LABEL:
@@ -213,16 +211,16 @@ val OBS_RESTR_PR_LAB_NIL = save_thm (
 val OBS_RESTR_PREFIX_LABEL = save_thm (
    "OBS_RESTR_PREFIX_LABEL",
   ((Q.GENL [`l`, `L`]) o
-   (DISCH ``~((l :'b Label) IN L) /\ ~((COMPL l) IN L)``) o
+   (DISCH ``~((l :'a Label) IN L) /\ ~((COMPL l) IN L)``) o
    (Q.GEN `E`) o
    UNDISCH)
       (IMP_TRANS
-           (DISCH ``~((l :'b Label) IN L) /\ ~((COMPL l) IN L)``
+           (DISCH ``~((l :'a Label) IN L) /\ ~((COMPL l) IN L)``
             (Q.SPEC `E`
              (UNDISCH
               (Q.SPECL [`l`, `L`] STRONG_RESTR_PREFIX_LABEL))))
-           (SPECL [``restr (L :'b Label set) (prefix (label l) E)``,
-                   ``prefix (label (l :'b Label)) (restr L E)``]
+           (SPECL [``restr (L :'a Label set) (prefix (label l) E)``,
+                   ``prefix (label (l :'a Label)) (restr L E)``]
                   STRONG_IMP_OBS_CONGR)));
 
 (******************************************************************************)
@@ -288,7 +286,7 @@ val OBS_RELAB_PREFIX = save_thm (
    |- !u E. OBS_CONGR (prefix u (prefix tau E)) (prefix u E)
  *)
 val TAU1 = store_thm ("TAU1",
-  ``!(u :'b Action) E. OBS_CONGR (prefix u (prefix tau E)) (prefix u E)``,
+  ``!(u :'a Action) E. OBS_CONGR (prefix u (prefix tau E)) (prefix u E)``,
     REPEAT GEN_TAC
  >> PURE_ONCE_REWRITE_TAC [OBS_CONGR]
  >> REPEAT STRIP_TAC (* 2 sub-goals here *)
@@ -296,15 +294,15 @@ val TAU1 = store_thm ("TAU1",
       IMP_RES_TAC TRANS_PREFIX \\
       Q.EXISTS_TAC `E` \\
       ASM_REWRITE_TAC [WEAK_TRANS, TAU_WEAK] \\
-      EXISTS_TAC ``prefix (u :'b Action) E`` \\
+      EXISTS_TAC ``prefix (u :'a Action) E`` \\
       Q.EXISTS_TAC `E` \\
       ASM_REWRITE_TAC [EPS_REFL, PREFIX],
       (* goal 2 (of 2) *)
       IMP_RES_TAC TRANS_PREFIX \\
-      EXISTS_TAC ``prefix (tau :'b Action) E2`` \\
+      EXISTS_TAC ``prefix (tau :'a Action) E2`` \\
       ASM_REWRITE_TAC [WEAK_TRANS, TAU_WEAK] \\
-      EXISTS_TAC ``prefix (u :'b Action) (prefix tau E2)`` \\
-      EXISTS_TAC ``prefix (tau :'b Action) E2`` \\
+      EXISTS_TAC ``prefix (u :'a Action) (prefix tau E2)`` \\
+      EXISTS_TAC ``prefix (tau :'a Action) E2`` \\
       ASM_REWRITE_TAC [EPS_REFL, PREFIX] ]);
 
 (* Prove WEAK_TAU1:
@@ -356,7 +354,7 @@ val WEAK_TAU2 = save_thm ("WEAK_TAU2",
                  (prefix u (sum E (prefix tau E')))
  *)
 val TAU3 = store_thm ("TAU3",
-  ``!(u :'b Action) E E'.
+  ``!(u :'a Action) E E'.
         OBS_CONGR (sum (prefix u (sum E (prefix tau E'))) (prefix u E'))
                   (prefix u (sum E (prefix tau E')))``,
     REPEAT GEN_TAC
@@ -373,7 +371,7 @@ val TAU3 = store_thm ("TAU3",
         IMP_RES_TAC TRANS_PREFIX \\
         Q.EXISTS_TAC `E1` \\
         ASM_REWRITE_TAC [WEAK_TRANS, WEAK_EQUIV_REFL] \\
-        take [`prefix (u :'b Action) (sum E (prefix tau E'))`,
+        take [`prefix (u :'a Action) (sum E (prefix tau E'))`,
               `sum E (prefix tau E')`] \\
         REWRITE_TAC [EPS_REFL, PREFIX] \\
         MATCH_MP_TAC ONE_TAU \\
