examples/CCS/WeakLawsScript.sml
@@ -6,8 +6,9 @@
 open HolKernel Parse boolLib bossLib;
 
 open pred_setTheory prim_recTheory arithmeticTheory relationTheory;
-open CCSLib CCSTheory StrongEQTheory StrongLawsTheory;
-open WeakEQTheory WeakEQLib;
+
+open CCSLib CCSTheory StrongEQTheory StrongLawsTheory
+     WeakEQTheory WeakEQLib;
 
 val _ = new_theory "WeakLaws";
 
@@ -139,7 +140,7 @@ val WEAK_PAR_TAU_TAU = save_thm (
  *)
 val WEAK_PAR_PREF_NO_SYNCR = save_thm (
    "WEAK_PAR_PREF_NO_SYNCR",
-    STRIP_FORALL_RULE ((DISCH ``~((l :'b Label) = COMPL l')``) o
+    STRIP_FORALL_RULE ((DISCH ``~((l :'a Label) = COMPL l')``) o
                        (STRONG_IMP_WEAK_EQUIV_RULE) o
                        UNDISCH)
                       STRONG_PAR_PREF_NO_SYNCR);
@@ -156,7 +157,7 @@ val WEAK_PAR_PREF_NO_SYNCR = save_thm (
  *)
 val WEAK_PAR_PREF_SYNCR = save_thm (
    "WEAK_PAR_PREF_SYNCR",
-    STRIP_FORALL_RULE ((DISCH ``((l :'b Label) = COMPL l')``) o
+    STRIP_FORALL_RULE ((DISCH ``((l :'a Label) = COMPL l')``) o
                        (STRONG_IMP_WEAK_EQUIV_RULE) o
                        UNDISCH)
                       STRONG_PAR_PREF_SYNCR);
@@ -211,15 +212,15 @@ val WEAK_RESTR_PREFIX_TAU = save_thm (
 val WEAK_RESTR_PR_LAB_NIL = save_thm (
    "WEAK_RESTR_PR_LAB_NIL",
     GEN_ALL
-       (DISCH ``(l :'b Label) IN L \/ (COMPL l) IN L``
+       (DISCH ``(l :'a Label) IN L \/ (COMPL l) IN L``
         (Q.GEN `E`
          (UNDISCH
           (IMP_TRANS
-           (DISCH ``(l :'b Label) IN L \/ (COMPL l) IN L``
+           (DISCH ``(l :'a Label) IN L \/ (COMPL l) IN L``
             (Q.SPEC `E`
              (UNDISCH
               (Q.SPECL [`l`, `L`] STRONG_RESTR_PR_LAB_NIL))))
-           (SPECL [``restr (L :'b Label set) (prefix (label l) E)``, ``nil``]
+           (SPECL [``restr (L :'a Label set) (prefix (label l) E)``, ``nil``]
                     STRONG_IMP_WEAK_EQUIV))))));
 
 (* Prove WEAK_RESTR_PREFIX_LABEL:
@@ -230,16 +231,16 @@ val WEAK_RESTR_PR_LAB_NIL = save_thm (
 val WEAK_RESTR_PREFIX_LABEL = save_thm (
    "WEAK_RESTR_PREFIX_LABEL",
     GEN_ALL
-       (DISCH ``~((l :'b Label) IN L) /\ ~((COMPL l) IN L)``
+       (DISCH ``~((l :'a Label) IN L) /\ ~((COMPL l) IN L)``
         (Q.GEN `E`
          (UNDISCH
           (IMP_TRANS
-           (DISCH ``~((l :'b Label) IN L) /\ ~((COMPL l) IN L)``
+           (DISCH ``~((l :'a Label) IN L) /\ ~((COMPL l) IN L)``
             (Q.SPEC `E`
              (UNDISCH
               (Q.SPECL [`l`, `L`] STRONG_RESTR_PREFIX_LABEL))))
-           (SPECL [``restr (L :'b Label set) (prefix (label l) E)``,
-                   ``prefix (label (l :'b Label)) (restr L E)``]
+           (SPECL [``restr (L :'a Label set) (prefix (label l) E)``,
+                   ``prefix (label (l :'a Label)) (restr L E)``]
                   STRONG_IMP_WEAK_EQUIV))))));
 
 (******************************************************************************)
